books/kestrel/remora/type-equivalence.lisp
@@ -50,64 +50,101 @@
 
 ;;;;;;;;;;;;;;;;;;;;;;;;;;;;;;;;;;;;;;;;;;;;;;;;;;;;;;;;;;;;;;;;;;;;;;;;;;;;;;;;
 
-(define check-ispace-var-renaming ((params1 ispace-var-listp)
-                                   (params2 ispace-var-listp))
+(define check-ispace-var-renaming ((vars1 ispace-var-listp)
+                                   (vars2 ispace-var-listp))
   :returns (dim-and-shape-maps stringstringmap-pair-resultp)
   :short "Check if two lists of ispace variables match in number and sorts,
           and if so return maps between the dimension and shape variables."
-  (b* (((when (endp params1))
-        (if (endp params2)
+  (b* (((when (endp vars1))
+        (if (endp vars2)
             (make-stringstringmap-pair :1st nil :2nd nil)
           (reserr nil)))
-       ((when (endp params2)) (reserr nil))
+       ((when (endp vars2)) (reserr nil))
        ((ok (stringstringmap-pair maps))
-        (check-ispace-var-renaming (cdr params1) (cdr params2)))
-       (param1 (car params1))
-       (param2 (car params2)))
+        (check-ispace-var-renaming (cdr vars1) (cdr vars2)))
+       (var1 (car vars1))
+       (var2 (car vars2)))
     (ispace-var-case
-     param1
+     var1
      :dim (ispace-var-case
-           param2
+           var2
            :dim (make-stringstringmap-pair
-                 :1st (omap::update param1.name param2.name maps.1st)
+                 :1st (omap::update var1.name var2.name maps.1st)
                  :2nd maps.2nd)
            :shape (reserr nil))
      :shape (ispace-var-case
-             param2
+             var2
              :dim (reserr nil)
              :shape (make-stringstringmap-pair
                      :1st maps.1st
-                     :2nd (omap::update param1.name param2.name maps.2nd)))))
+                     :2nd (omap::update var1.name var2.name maps.2nd)))))
+  :verify-guards :after-returns)
+
+;;;;;;;;;;;;;;;;;;;;;;;;;;;;;;;;;;;;;;;;
+
+(define check-type-var-renaming ((vars1 type-var-listp)
+                                 (vars2 type-var-listp))
+  :returns (atom-and-array-maps stringstringmap-pair-resultp)
+  :short "Check if two lists of type variables match in number and kinds,
+          and if so return maps between the atom and array variables."
+  (b* (((when (endp vars1))
+        (if (endp vars2)
+            (make-stringstringmap-pair :1st nil :2nd nil)
+          (reserr nil)))
+       ((when (endp vars2)) (reserr nil))
+       ((ok (stringstringmap-pair maps))
+        (check-type-var-renaming (cdr vars1) (cdr vars2)))
+       (var1 (car vars1))
+       (var2 (car vars2)))
+    (type-var-case
+     var1
+     :atom (type-var-case
+            var2
+            :atom (make-stringstringmap-pair
+                   :1st (omap::update var1.name var2.name maps.1st)
+                   :2nd maps.2nd)
+            :array (reserr nil))
+     :array (type-var-case
+             var2
+             :atom (reserr nil)
+             :array (make-stringstringmap-pair
+                     :1st maps.1st
+                     :2nd (omap::update var1.name var2.name maps.2nd)))))
   :verify-guards :after-returns)
 
 ;;;;;;;;;;;;;;;;;;;;;;;;;;;;;;;;;;;;;;;;;;;;;;;;;;;;;;;;;;;;;;;;;;;;;;;;;;;;;;;;
 
-(defines types-renamep
-  :short "Check if two types or lists or types are the same modulo renaming."
+(defines atom/array-types-renamep
+  :short "Check if two atom types, array types, or lists of array types
+          are the same modulo renaming."
   :long
   (xdoc::topstring
    (xdoc::p
-    "There are three independent renamings:
+    "There are four independent renamings:
      one for dimension variables,
      one for shape variables,
-     and one for type variables.
+     one for atom type variables, and
+     one for array type variables.
      These are modeled as maps from strings to strings,
      which should be injective
      in well-formed types according to inference rules;
      we may explicate injectivity as guards and invariants at some point.
-     The three renaming maps contain all the variables in scope;
+     The four renaming maps contain all the variables in scope;
      we should explicate this invariant at some point;
      some variables may be associated to themselves (i.e. not renamed)
      in the renaming maps."))
 
-  (define type-renamep ((type1 typep)
-                        (type2 typep)
-                        (dim-renaming string-string-mapp)
-                        (shape-renaming string-string-mapp)
-                        (type-renaming string-string-mapp))
+  ;;;;;;;;;;;;;;;;;;;;;;;;;;;;;;;;;;;;;;;;
+
+  (define atom-type-renamep ((type1 atom-typep)
+                             (type2 atom-typep)
+                             (dim-renam string-string-mapp)
+                             (shape-renam string-string-mapp)
+                             (atom-renam string-string-mapp)
+                             (array-renam string-string-mapp))
     :returns (yes/no booleanp)
-    :parents (type-equivalence types-renamep)
-    :short "Check if two types are the same modulo renaming."
+    :parents (type-equivalence atom/array-types-renamep)
+    :short "Check if two atom types are the same modulo renaming."
     :long
     (xdoc::topstring
      (xdoc::p
@@ -122,208 +159,324 @@
       "In the case of two base types,
        they must be identical, because they do not contain variables.")
      (xdoc::p
-      "In the case of two array types,
-       we recursively check the equality modulo renaming of the atom types.
-       For the shapes,
-       first we apply the dimension and shape variable renaming
-       to the first shape,
-       and then we check equivalence with the second shape.
-       Shape equivalence is defined not modulo renaming,
-       so we must apply the renaming prior to checking shape equivalence.")
-     (xdoc::p
       "In the case of two function types,
        we recursively check the equality modulo renaming
        of the input and output types.")
      (xdoc::p
       "In the case of two universal types,
-       we check that they have the same number of bound variables,
-       and we form a map between their bound variables,
-       with which we update the existing type variable renaming map;
+       we use a separate function to check that
+       they have the same number and kinds of bound variables,
+       forming two maps between their bound variables,
+       one for atom variables and one for array variables,
+       with which we update the existing variable renaming maps;
        this update may overwrite some previous associations,
        in line with the fact that the bound variables
        may hide outer variables.
-       We then check that the two inner types are equal
+       We then check that the two body types are equal
        modulo the updated renamings.")
      (xdoc::p
       "In the case of two product types or two sum types,
        we use a separate function to check that
-       they have the same number and sorte of bound variables,
+       they have the same number and sorts of bound variables,
        forming two maps between their bound variables,
        one for dimension variables and one for shape variables,
        with which we update the existing variable renaming maps;
        this update may overwrite some previous associations,
        in line with the fact that the bound variables
        may hide outer variables.
-       We then check that the two inner types are equal
+       We then check that the two body types are equal
        modulo the updated renamings."))
-    (type-case
+    (atom-type-case
      type1
-     :var (type-case
+     :var (atom-type-case
            type2
-           :var (b* ((type-renaming (string-string-map-fix type-renaming)))
-                  (equal (omap::assoc type1.name type-renaming)
+           :var (b* ((atom-renam (string-string-map-fix atom-renam)))
+                  (equal (omap::assoc type1.name atom-renam)
                          (cons type1.name type2.name)))
            :otherwise nil)
-     :base (type-case
+     :base (atom-type-case
             type2
             :base (equal type1.type type2.type)
             :otherwise nil)
-     :array (type-case
-             type2
-             :array (and (type-renamep type1.type
-                                       type2.type
-                                       dim-renaming
-                                       shape-renaming
-                                       type-renaming)
-                         (b* ((renamed-shape1
-                               (shape-rename-ispace-vars type1.shape
-                                                         dim-renaming
-                                                         shape-renaming)))
-                           (shape-equivp renamed-shape1 type2.shape)))
-             :otherwise nil)
-     :fun (type-case
+     :fun (atom-type-case
            type2
-           :fun (and (type-list-renamep type1.in
-                                        type2.in
-                                        dim-renaming
-                                        shape-renaming
-                                        type-renaming)
-                     (type-renamep type1.out
-                                   type2.out
-                                   dim-renaming
-                                   shape-renaming
-                                   type-renaming))
+           :fun (and (array-type-list-renamep type1.in
+                                              type2.in
+                                              dim-renam
+                                              shape-renam
+                                              atom-renam
+                                              array-renam)
+                     (array-type-renamep type1.out
+                                         type2.out
+                                         dim-renam
+                                         shape-renam
+                                         atom-renam
+                                         array-renam))
            :otherwise nil)
-     :forall (type-case
+     :forall (atom-type-case
               type2
-              :forall (and (equal (len type1.vars) (len type2.vars))
-                           (b* ((bound-map (omap::from-lists
-                                            (kinded-var-list->var type1.vars)
-                                            (kinded-var-list->var type2.vars)))
-                                (type-renaming
-                                 (omap::update*
-                                  bound-map
-                                  (string-string-map-fix type-renaming))))
-                             (type-renamep type1.type
-                                           type2.type
-                                           dim-renaming
-                                           shape-renaming
-                                           type-renaming)))
+              :forall (b* ((maps (check-type-var-renaming type1.params
+                                                          type2.params))
+                           ((when (reserrp maps)) nil)
+                           ((stringstringmap-pair maps) maps)
+                           (atom-renam (omap::update*
+                                        maps.1st
+                                        (string-string-map-fix atom-renam)))
+                           (array-renam (omap::update*
+                                         maps.2nd
+                                         (string-string-map-fix array-renam))))
+                        (array-type-renamep type1.type
+                                            type2.type
+                                            dim-renam
+                                            shape-renam
+                                            atom-renam
+                                            array-renam))
               :otherwise nil)
-     :pi (type-case
+     :pi (atom-type-case
           type2
           :pi (b* ((maps (check-ispace-var-renaming type1.params
                                                     type2.params))
                    ((when (reserrp maps)) nil)
                    ((stringstringmap-pair maps) maps)
-                   (dim-renaming (omap::update*
-                                  maps.1st
-                                  (string-string-map-fix dim-renaming)))
-                   (shape-renaming (omap::update*
-                                    maps.2nd
-                                    (string-string-map-fix shape-renaming))))
-                (type-renamep type1.type
-                              type2.type
-                              dim-renaming
-                              shape-renaming
-                              type-renaming))
+                   (dim-renam (omap::update*
+                               maps.1st
+                               (string-string-map-fix dim-renam)))
+                   (shape-renam (omap::update*
+                                 maps.2nd
+                                 (string-string-map-fix shape-renam))))
+                (array-type-renamep type1.type
+                                    type2.type
+                                    dim-renam
+                                    shape-renam
+                                    atom-renam
+                                    array-renam))
           :otherwise nil)
-     :sigma (type-case
+     :sigma (atom-type-case
              type2
              :sigma (b* ((maps (check-ispace-var-renaming type1.params
                                                           type2.params))
                          ((when (reserrp maps)) nil)
                          ((stringstringmap-pair maps) maps)
-                         (dim-renaming (omap::update*
-                                        maps.1st
-                                        (string-string-map-fix dim-renaming)))
-                         (shape-renaming (omap::update*
-                                          maps.2nd
-                                          (string-string-map-fix
-                                           shape-renaming))))
-                      (type-renamep type1.type
-                                    type2.type
-                                    dim-renaming
-                                    shape-renaming
-                                    type-renaming))
+                         (dim-renam (omap::update*
+                                     maps.1st
+                                     (string-string-map-fix dim-renam)))
+                         (shape-renam (omap::update*
+                                       maps.2nd
+                                       (string-string-map-fix shape-renam))))
+                      (array-type-renamep type1.type
+                                          type2.type
+                                          dim-renam
+                                          shape-renam
+                                          atom-renam
+                                          array-renam))
              :otherwise nil))
-    :measure (+ (type-count type1) (type-count type2)))
+    :measure (+ (atom-type-count type1) (atom-type-count type2)))
 
-  (define type-list-renamep ((types1 type-listp)
-                             (types2 type-listp)
-                             (dim-renaming string-string-mapp)
-                             (shape-renaming string-string-mapp)
-                             (type-renaming string-string-mapp))
+  ;;;;;;;;;;;;;;;;;;;;;;;;;;;;;;;;;;;;;;;;
+
+  (define array-type-renamep ((type1 array-typep)
+                              (type2 array-typep)
+                              (dim-renam string-string-mapp)
+                              (shape-renam string-string-mapp)
+                              (atom-renam string-string-mapp)
+                              (array-renam string-string-mapp))
     :returns (yes/no booleanp)
-    :parents (type-equivalence types-renamep)
-    :short "Check if two lists of types are the same modulo renaming."
+    :parents (type-equivalence atom/array-types-renamep)
+    :short "Check if two array types are the same modulo renaming."
+    :long
+    (xdoc::topstring
+     (xdoc::p
+      "The two types must be in the same fixtype summand:
+       two variables, or two explicit array types.")
+     (xdoc::p
+      "In the case of two variables,
+       since the renaming contains all the variables in scope,
+       we check that the first and second variables
+       are associated in the renaming map.")
+     (xdoc::p
+      "In the case of two explicit array types,
+       we recursively check the equality modulo renaming of the body types.
+       For the shapes,
+       first we apply the dimension and shape variable renaming
+       to the first shape,
+       and then we check equivalence with the second shape.
+       Shape equivalence is defined not modulo renaming,
+       so we must apply the renaming prior to checking shape equivalence."))
+    (array-type-case
+     type1
+     :var (array-type-case
+           type2
+           :var (b* ((array-renam (string-string-map-fix array-renam)))
+                  (equal (omap::assoc type1.name array-renam)
+                         (cons type1.name type2.name)))
+           :otherwise nil)
+     :array (array-type-case
+             type2
+             :array (and (atom-type-renamep type1.type
+                                            type2.type
+                                            dim-renam
+                                            shape-renam
+                                            atom-renam
+                                            array-renam)
+                         (b* ((renamed-shape1
+                               (shape-rename-ispace-vars type1.shape
+                                                         dim-renam
+                                                         shape-renam)))
+                           (shape-equivp renamed-shape1 type2.shape)))
+             :otherwise nil))
+    :measure (+ (array-type-count type1) (array-type-count type2)))
+
+  ;;;;;;;;;;;;;;;;;;;;;;;;;;;;;;;;;;;;;;;;
+
+  (define array-type-list-renamep ((types1 array-type-listp)
+                                   (types2 array-type-listp)
+                                   (dim-renam string-string-mapp)
+                                   (shape-renam string-string-mapp)
+                                   (atom-renam string-string-mapp)
+                                   (array-renam string-string-mapp))
+    :returns (yes/no booleanp)
+    :parents (type-equivalence atom/array-types-renamep)
+    :short "Check if two lists of array types are the same modulo renaming."
     (or (and (endp types1)
              (endp types2))
         (and (consp types1)
              (consp types2)
-             (type-renamep (car types1)
-                           (car types2)
-                           dim-renaming
-                           shape-renaming
-                           type-renaming)
-             (type-list-renamep (cdr types1)
-                                (cdr types2)
-                                dim-renaming
-                                shape-renaming
-                                type-renaming)))
-    :measure (+ (type-list-count types1) (type-list-count types2))
+             (array-type-renamep (car types1)
+                                 (car types2)
+                                 dim-renam
+                                 shape-renam
+                                 atom-renam
+                                 array-renam)
+             (array-type-list-renamep (cdr types1)
+                                      (cdr types2)
+                                      dim-renam
+                                      shape-renam
+                                      atom-renam
+                                      array-renam)))
+    :measure (+ (array-type-list-count types1) (array-type-list-count types2))
 
     ///
 
-    (defrule same-len-when-type-list-renamep
-      (implies (type-list-renamep
-                types1 types2 dim-renaming shape-renaming type-renaming)
+    (defrule same-len-when-array-type-list-renamep
+      (implies (array-type-list-renamep types1
+                                        types2
+                                        dim-renam
+                                        shape-renam
+                                        atom-renam
+                                        array-renam)
                (equal (len types1) (len types2)))
       :rule-classes :forward-chaining
       :hints (("Goal"
                :induct (acl2::cdr-cdr-induct types1 types2)
                :in-theory (enable acl2::atom)))))
 
+  ;;;;;;;;;;;;;;;;;;;;;;;;;;;;;;;;;;;;;;;;
+
   ///
 
-  (fty::deffixequiv-mutual types-renamep))
-
-;;;;;;;;;;;;;;;;;;;;;;;;;;;;;;;;;;;;;;;;;;;;;;;;;;;;;;;;;;;;;;;;;;;;;;;;;;;;;;;;
-
-(define type-equivp ((type1 typep) (type2 typep))
-  :returns (yes/no booleanp)
-  :short "Check if two types are equivalent."
-  :long
-  (xdoc::topstring
-   (xdoc::p
-    "This is the case when they are equal modulo no renamings."))
-  (type-renamep type1 type2 nil nil nil))
+  (fty::deffixequiv-mutual atom/array-types-renamep))
 
 ;;;;;;;;;;;;;;;;;;;;;;;;;;;;;;;;;;;;;;;;
 
-(define type-list-equivp ((types1 type-listp) (types2 type-listp))
+(define atom-type-list-renamep ((types1 atom-type-listp)
+                                (types2 atom-type-listp)
+                                (dim-renam string-string-mapp)
+                                (shape-renam string-string-mapp)
+                                (atom-renam string-string-mapp)
+                                (array-renam string-string-mapp))
   :returns (yes/no booleanp)
-  :short "Check if two lists of types are equivalent."
+  :short "Check if two lists of atom types are the same modulo renaming."
+  (or (and (endp types1)
+           (endp types2))
+      (and (consp types1)
+           (consp types2)
+           (atom-type-renamep (car types1)
+                              (car types2)
+                              dim-renam
+                              shape-renam
+                              atom-renam
+                              array-renam)
+           (atom-type-list-renamep (cdr types1)
+                                   (cdr types2)
+                                   dim-renam
+                                   shape-renam
+                                   atom-renam
+                                   array-renam)))
+
+  ///
+
+  (defrule same-len-when-atom-type-list-renamep
+    (implies (atom-type-list-renamep types1
+                                     types2
+                                     dim-renam
+                                     shape-renam
+                                     atom-renam
+                                     array-renam)
+             (equal (len types1) (len types2)))
+    :rule-classes :forward-chaining
+    :hints (("Goal"
+             :induct (acl2::cdr-cdr-induct types1 types2)
+             :in-theory (enable acl2::atom)))))
+
+;;;;;;;;;;;;;;;;;;;;;;;;;;;;;;;;;;;;;;;;;;;;;;;;;;;;;;;;;;;;;;;;;;;;;;;;;;;;;;;;
+
+(define atom-type-equivp ((type1 atom-typep) (type2 atom-typep))
+  :returns (yes/no booleanp)
+  :short "Check if two atom types are equivalent."
   :long
   (xdoc::topstring
    (xdoc::p
     "This is the case when they are equal modulo no renamings."))
-  (type-list-renamep types1 types2 nil nil nil)
+  (atom-type-renamep type1 type2 nil nil nil nil))
+
+;;;;;;;;;;;;;;;;;;;;
+
+(define atom-type-list-equivp ((types1 atom-type-listp)
+                               (types2 atom-type-listp))
+  :returns (yes/no booleanp)
+  :short "Check if two lists of atom types are equivalent."
+  :long
+  (xdoc::topstring
+   (xdoc::p
+    "This is the case when they are equal modulo no renamings."))
+  (atom-type-list-renamep types1 types2 nil nil nil nil)
 
   ///
 
-  (defrule same-len-when-type-list-equivp
-    (implies (type-list-equivp types1 types2)
+  (defrule same-len-when-atom-type-list-equivp
+    (implies (atom-type-list-equivp types1 types2)
              (equal (len types1) (len types2)))
     :rule-classes :forward-chaining))
 
+;;;;;;;;;;;;;;;;;;;;;;;;;;;;;;;;;;;;;;;;
+
+(define array-type-equivp ((type1 array-typep) (type2 array-typep))
+  :returns (yes/no booleanp)
+  :short "Check if two array types are equivalent."
+  :long
+  (xdoc::topstring
+   (xdoc::p
+    "This is the case when they are equal modulo no renamings."))
+  (array-type-renamep type1 type2 nil nil nil nil))
+
 ;;;;;;;;;;;;;;;;;;;;;;;;;;;;;;;;;;;;;;;;;;;;;;;;;;;;;;;;;;;;;;;;;;;;;;;;;;;;;;;;
 
-(define type-list-all-equivp ((types type-listp))
+(define atom-type-list-all-equivp ((types atom-type-listp))
   :returns (yes/no booleanp)
-  :short "Check if all the types in a list are equivalent."
+  :short "Check if all the atom types in a list are equivalent."
   (or (endp types)
       (endp (cdr types))
-      (and (type-equivp (car types) (cadr types))
-           (type-list-all-equivp (cdr types))))
-  :prepwork ((local (in-theory (enable type-list-fix)))))
+      (and (atom-type-equivp (car types) (cadr types))
+           (atom-type-list-all-equivp (cdr types))))
+  :prepwork ((local (in-theory (enable atom-type-list-fix)))))
+
+;;;;;;;;;;;;;;;;;;;;;;;;;;;;;;;;;;;;;;;;
+
+(define array-type-list-all-equivp ((types array-type-listp))
+  :returns (yes/no booleanp)
+  :short "Check if all the array types in a list are equivalent."
+  (or (endp types)
+      (endp (cdr types))
+      (and (array-type-equivp (car types) (cadr types))
+           (array-type-list-all-equivp (cdr types))))
+  :prepwork ((local (in-theory (enable array-type-list-fix)))))
